S2I/Compiler.v
@@ -10,42 +10,13 @@ Open Scope monad_scope.
 
 Record comp_env : Type := {
   next_label: label;
-  current_component : Component.id;
-  local_buffers : PMap.t (list Block.id);
-  procs_labels : PMap.t (PMap.t label)
+  (* facts about this? *)
 }.
 
 (* easy environments updates *)
 
-Definition with_next_label l env :=
-  {| next_label := l;
-     current_component := current_component env;
-     local_buffers := local_buffers env;
-     procs_labels := procs_labels env |}.
-
-Definition with_current_component C env :=
-  {| next_label := next_label env;
-     current_component := C;
-     local_buffers := local_buffers env;
-     procs_labels := procs_labels env |}.
-
-Definition with_component_buffers C bufs env :=
-  {| next_label := next_label env;
-     current_component := current_component env;
-     local_buffers := PMap.add C bufs (local_buffers env);
-     procs_labels := procs_labels env |}.
-
-Definition with_new_proc_label C P l env :=
-  {| next_label := next_label env;
-     current_component := current_component env;
-     local_buffers := local_buffers env;
-     procs_labels :=
-       let proc_labels' :=
-           match PMap.find C (procs_labels env) with
-           | None => PMap.add P l (@PMap.empty label)
-           | Some labels => PMap.add P l labels
-           end
-       in PMap.add C proc_labels' (procs_labels env) |}.
+Definition with_next_label l (env:comp_env) :=
+  {| next_label := l; |}.
 
 (* simplify notations *)
 
@@ -64,25 +35,6 @@ Definition fresh_label : COMP label :=
   let l := next_label cenv in
   do! modify (with_next_label (1+l)%positive);
   ret l.
-
-Definition get_local_buffer : COMP Pointer.t :=
-  do cenv <- get;
-  let C := current_component cenv in
-  do blocks <- lift (PMap.find C (local_buffers cenv));
-  do b <- lift (nth_error blocks 0);
-  ret (C, b, 0).
-
-Definition get_temp_buffer : COMP Pointer.t:=
-  do cenv <- get;
-  let C := current_component cenv in
-  do blocks <- lift (PMap.find C (local_buffers cenv));
-  do b <- lift (nth_error blocks (length blocks - 1));
-  ret (C, b, 0).
-
-Definition find_proc_label C P : COMP label :=
-  do cenv <- get;
-  do P_labels <- lift (PMap.find C (procs_labels cenv));
-  lift (PMap.find P P_labels).
 
 (* code generation *)
 
@@ -117,6 +69,16 @@ Definition restore_environment (buf: Pointer.t) : code :=
   IConst (IInt 1) R_ONE ::
   restore_stack_frame_pointer buf.
 
+Section WithComponent.
+
+Variable C: Component.id. (* the current component *)  
+Variable local_buf_ptr : Pointer.t. (* pointer to the local buffer for current component *)
+Variable temp_buf_ptr : Pointer.t.  (* pointer to the temp buffer for current component. *)
+Variable P_labels : PMap.t label.  (* map from procedure id's to start labels for current component *)
+
+Definition find_proc_label P : COMP label :=
+  lift (PMap.find P P_labels).
+
 Fixpoint compile_expr (e: expr) : COMP code :=
   match e with
   | E_val (Int i) =>
@@ -125,7 +87,6 @@ Fixpoint compile_expr (e: expr) : COMP code :=
     ret [IConst (IPtr p) R_COM]
   | E_val Undef => fail (* we don't compile undef *)
   | E_local =>
-    do local_buf_ptr <- get_local_buffer;
     ret [IConst (IPtr local_buf_ptr) R_COM]
   | E_binop bop e1 e2 =>
     do c1 <- compile_expr e1;
@@ -169,12 +130,9 @@ Fixpoint compile_expr (e: expr) : COMP code :=
          pop R_AUX1 ++
          IStore R_COM R_AUX1 :: nil)
   | E_call C' P' e =>
-    do cenv <- get;
-    let C := current_component cenv in
-    do local_buf_ptr <- get_local_buffer;
     do call_arg_code <- compile_expr e;
     if Pos.eqb C' C then
-      do target_label <- find_proc_label C' P';
+      do target_label <- find_proc_label P';
       ret (call_arg_code ++
            push R_AUX2 ++
            load_arg local_buf_ptr R_AUX1 ++
@@ -184,7 +142,6 @@ Fixpoint compile_expr (e: expr) : COMP code :=
            store_arg local_buf_ptr R_AUX1 R_AUX2 ++
            pop R_AUX2)
     else
-      do temp_buf_ptr <- get_temp_buffer;
       ret (call_arg_code ++
            push R_AUX2 ++
            load_arg local_buf_ptr R_AUX1 ++
@@ -198,12 +155,10 @@ Fixpoint compile_expr (e: expr) : COMP code :=
   | E_exit => ret [IHalt]
   end.
 
-Definition compile_proc
-           (C: Component.id) (P: Procedure.id) (e: expr)
+
+Definition compile_proc (P: Procedure.id) (e: expr)
   : COMP code :=
-  do! modify (with_current_component C);
-  do proc_label <- find_proc_label C P;
-  do local_buf_ptr <- get_local_buffer;
+  do proc_label <- find_proc_label P;
   do lmain <- fresh_label;
   do lreturn <- fresh_label;
   do proc_code <- compile_expr e;
@@ -231,84 +186,116 @@ Definition compile_proc
         ILabel lreturn;
         IReturn]).
 
-Fixpoint gen_component_procedures_labels
-         (C: Component.id) (procs: list (Procedure.id * expr))
-  : COMP unit :=
-  match procs with
-  | [] => ret tt
-  | (P, _) :: procs' =>
-    do freshl <- fresh_label;
-    do! modify (with_new_proc_label C P freshl);
-    gen_component_procedures_labels C procs'
-  end.
-
-(* think about labels collision when linking partial programs *)
-Fixpoint gen_all_procedures_labels
-         (procs: list (Component.id * PMap.t expr))
-  : COMP unit :=
-  match procs with
-  | [] => ret tt
-  | (C, Cprocs) :: procs' =>
-    do! gen_component_procedures_labels C (PMap.elements Cprocs);
-    gen_all_procedures_labels procs'
-  end.
-
-Fixpoint add_temporary_buffers
-         (bufs: list (Component.id * nat))
-  : COMP (PMap.t (list (Block.id * nat))) :=
-  let fix instrument acc bs :=
-      match bs with
-      | [] => ret acc
-      | (C,size) :: bs' =>
-        let Cbufs := [(1%positive,size%nat); (2%positive,1%nat)] in
-        let acc' := PMap.add C Cbufs acc in
-        do! modify (with_component_buffers C (map fst Cbufs));
-        instrument acc' bs'
-      end
-  in instrument (PMap.empty (list (Block.id * nat))) bufs.
-
-Fixpoint compile_procedures
-         (C: Component.id)
+Definition compile_procedures
          (procs: list (Procedure.id * expr))
   : COMP (list (Procedure.id * code)) :=
   let fix compile acc ps :=
       match ps with
       | [] => ret acc
       | (P,e) :: ps' =>
-        do proc_code <- compile_proc C P e;
+        do proc_code <- compile_proc P e;
         let acc' := (P,proc_code) :: acc in
         compile acc' ps'
       end
   in compile [] procs.
 
-Fixpoint compile_components
+End WithComponent.
+
+Definition gen_component_procedures_labels
+         (procs: list (Procedure.id * expr))
+  : COMP (PMap.t label) :=
+  let fix gen acc procs := 
+      match procs with
+      | [] => ret acc 
+      | (P, _) :: procs' =>
+        do freshl <- fresh_label;
+          gen (PMap.add P freshl acc) procs'
+      end
+  in gen (@PMap.empty label) procs.
+
+(* think about labels collision when linking partial programs *)
+Definition gen_all_procedures_labels
+         (procs: list (Component.id * PMap.t expr))
+  : COMP (PMap.t (PMap.t label)) :=
+  let fix gen acc procs := 
+      match procs with
+      | [] => ret acc 
+      | (C, Cprocs) :: procs' =>
+        do map <- gen_component_procedures_labels (PMap.elements Cprocs);
+          gen (PMap.add C map acc) procs'
+      end
+  in gen (@PMap.empty (PMap.t label)) procs.
+
+Definition add_temporary_buffers
+         (bufs: list (Component.id * nat))
+  : PMap.t (list (Block.id * nat)) :=
+  let fix instrument acc bs :=
+      match bs with
+      | [] => acc
+      | (C,size) :: bs' =>
+        let Cbufs := [(1%positive,size%nat); (2%positive,1%nat)] in
+        let acc' := PMap.add C Cbufs acc in
+        instrument acc' bs'
+      end
+  in instrument (PMap.empty (list (Block.id * nat))) bufs.
+
+Definition compile_components
+         (local_buffers : PMap.t (list (Block.id * nat)))
+         (procs_labels : PMap.t (PMap.t label))
          (comps: list (Component.id * PMap.t expr))
   : COMP (list (Component.id * PMap.t code)) :=
   let fix compile acc cs :=
       match cs with
       | [] => ret acc
       | (C,procs) :: cs' =>
-        do procs_code <- compile_procedures C (PMap.elements procs);
+        do blocks <- lift (PMap.find C local_buffers);
+        do local_buf <- lift (nth_error blocks 0);
+        do tmp_buf <- lift (nth_error blocks (length blocks - 1));
+        do P_labels <- lift (PMap.find C procs_labels);
+        do procs_code <- compile_procedures C (C,fst local_buf,0%Z) (C,fst tmp_buf,0%Z) P_labels (PMap.elements procs);
         let acc' := (C, PMapExtra.of_list procs_code) :: acc in
         compile acc' cs'
       end
   in compile [] comps.
 
 Definition init_env : comp_env :=
-  {| next_label := 1%positive;
-     current_component := 1%positive;
-     local_buffers := @PMap.empty (list Block.id);
-     procs_labels := @PMap.empty (PMap.t label) |}.
+  {| next_label := 1%positive; |}.
+
+
+(* In intermediate program, main will be a tiny wrapper routine (in the same component) 
+   that simply calls the  (translation of the) original main and then halts. *)
+
+(* A fresh procedure id can be calculated by, e.g., taking the max of all procedure id's and adding 1 *)
+Axiom generate_fresh_procedure_id : forall (procs: PMap.t (PMap.t code)), Procedure.id. 
+
+Definition wrap_main (procs_labels: PMap.t (PMap.t label)) (p: Intermediate.program) : COMP Intermediate.program :=
+  let '(C,P) := p.(Intermediate.prog_main) in
+  do iface <- lift (PMap.find C p.(Intermediate.prog_interface));
+  do procs <- lift (PMap.find C p.(Intermediate.prog_procedures));     
+  do P_labels <- lift (PMap.find C procs_labels); 
+  do lab <- lift (PMap.find P P_labels);
+  let P' := generate_fresh_procedure_id (p.(Intermediate.prog_procedures)) in
+  let iface' :=  {| Component.export := P'::iface.(Component.export);
+                    Component.import := iface.(Component.import) |} in
+  let procs' := PMap.add P' [IJal lab ; IHalt] procs in
+  ret 
+      {| Intermediate.prog_interface := PMap.add C iface' p.(Intermediate.prog_interface);
+         Intermediate.prog_procedures := PMap.add C procs' p.(Intermediate.prog_procedures);
+         Intermediate.prog_buffers := p.(Intermediate.prog_buffers);
+         Intermediate.prog_main := (C,P') |}
+.
 
 Definition compile_program
            (p: Source.program) : option Intermediate.program :=
-  let procs := PMap.elements (Source.prog_procedures p) in
+  let comps := PMap.elements (Source.prog_procedures p) in
   let bufs := PMap.elements (Source.prog_buffers p) in
+  let local_buffers := add_temporary_buffers bufs in  
   run init_env (
-    do! gen_all_procedures_labels procs;
-    do bufs' <- add_temporary_buffers bufs;
-    do code <- compile_components procs;
-    ret {| Intermediate.prog_interface := Source.prog_interface p;
+    do procs_labels <- gen_all_procedures_labels comps;
+    do code <- compile_components local_buffers procs_labels comps;
+    let p := 
+        {| Intermediate.prog_interface := Source.prog_interface p;
            Intermediate.prog_procedures := PMapExtra.of_list code;
-           Intermediate.prog_buffers := bufs';
-           Intermediate.prog_main := Source.prog_main p |}).
+           Intermediate.prog_buffers := local_buffers;
+           Intermediate.prog_main := Source.prog_main p |} in
+   wrap_main procs_labels p).
