S2I/Correctness.v
@@ -3,9 +3,9 @@ Require Import CompCert.Events.
 Require Import CompCert.Smallstep.
 Require Import CompCert.Behaviors.
 Require Import Source.Language.
-Require Source.CS.
+Require Import Source.CS.
 Require Import Intermediate.Machine.
-Require Intermediate.CS.
+Require Import Intermediate.CS.
 Require Import S2I.Compiler.
 Require Import S2I.Definitions.
 
@@ -82,6 +82,16 @@ forward simulation into a backward one.
 TODO prove determinacy and receptiveness
 *)
 
+Module S.
+  Import Source.CS.
+  Module CS := CS.
+End S.
+
+Module I.
+  Import Intermediate.CS.
+  Module CS := CS.
+End I.
+
 Section Correctness.
 Variable p: Source.program.
 Variable tp: Intermediate.program.
@@ -95,6 +105,391 @@ Hypothesis input_program_closedness:
 Hypothesis successful_compilation:
   compile_program p = Some tp.
 
+
+(* Some issues. 
+
++ Some outstanding questions about calling sequence.
++ Redesigning compilation to use a more minimal monad and add in the necessary uniqueness facts into the
+  monad type.
++ What about refactoring Source semantics to use an expression reduction function wherever possible?
+  Can't see what the continuation-based approach is buying except for divergence case.
+
+- Handling monad. (It should be simplified in any case to only track genuine state changes+error.)
+- Monad should also perhaps carry extension fact.
+- Maybe need a relational spec?  (cf rtlgen)
+- Will need to figure out how to carry fact about max stack size
+
+- Defining how memory changes:
+  + extra buffer for linkage
+  + extra dynamic buffer for stack
+- Defining stack relationship:
+  + source frames can be either local or remote target frames.
+
+Each subexpression of source corresponds to a contiguous sequence of machine code, which
+executes from top to bottom or (for exit) immediately halts.
+
+
+*)
+
+
+(* Relating states 
+
+s  = [old-C,old-call-arg,old-k]
+
+(C,s,mem,k,e)
+
+~
+
+gps  = [pointer]  -- return address into previous component.
+
+gps * mem * regs * pc 
+
+---------------
+
+relate_code e k pc
+
+evaluating (e,k) is equivalent to executing at pc up to... a halt(?)
+
+
+hugs
+  Inductive relate_states: sstate -> istate -> Prop :=
+  | rs_intro :  forall C s smem k e gps imem regs pc,
+      C = Pointer.component pc ->
+      relate_stacks s gps ->
+      relate_mems smem imem ->
+      relate_code e k (... pc) -> 
+      relate_state (C,s,smem,k,e) (gps,imem,regs,pc)
+.
+
+
+(* does it make sense to parameterize this by past memories and register sets?? *)
+(*  ?? doesn't make sense -- when are regs,mem captured?? *)
+Inductive relate_stacks (mem:Memory.t) : Component.id -> S.stack -> I.stack -> Pointer.t -> Pointer.t -> Prop :=
+  | rs_empty : forall sp0, relate_stacks mem nil nil sp0 sp0
+  | rs_diff_comp: 
+      relate_stacks C0 imem0 regs0 s0 gps spb0 sp0 ->
+      ((s0 = [] /\ C <> Main) \/ (exists C0, s0 = (C0,_,_)::_ /\ C <> C0)) ->
+      imem at sp0 contains an RA which is in sync with k0 and s (or whatever) ->
+      imem at sp0+1 contains arg ->
+      imem at spb contains sp0 -> 
+      imem at spb+1 contains arg  (* which was in locaxl buf ptr for C0 *) -> 
+      imem at (local buf ptr for C0) contains regs0(R_COM) -> maybe the current arg is just a parameter?
+      relate_stacks C imem ((C,arg,k)::s) ra??::gps spb (spb+??) ->  
+
+  | rs_same_comp : forall C0 arg0 k0 s gps spb0 sp0 -> 
+      relate_stacks mem s0 gps spb0 sp0 ->
+      ((s0 = [] /\ C == Main) \/ (s0 = (C,_,_)::_) -> 
+      imem at sp0 contains an RA which is in sync with k0 and s ?? -> 
+      -or ??? -- imem at sp0 contains regs0(RA) ->  ???
+      (* (imem at spb contains a block of appropriate stack_frame_sizep) -> *)
+      imem at spb contains sp0 -> 
+      imem at spb+1 contains arg  (* which was in local buf ptr for C0 *) -> 
+      imem at (local buf ptr for C0) contains regs0(R_COM) -> maybe the current arg is just a parameter?
+      XXX where are arg and k ??? 
+      relate_stacks imem ((C0,arg,k)::s) gps spb (spb+2)
+.
+
+(* What does code generated from an expression do?  
+
+Inductive tr_expr (G: Intermediate.GlobalEnv.global_env) :
+       Pointer.t -> nat -> expr -> Prop :=
+  | tr_expr run ->       
+       codeseq_at G pc0 n = c ->
+       c = translation of e -> 
+       .... -> 
+       tr_expr G pc0 n e
+  | tr_expr_halt: 
+       code_at G pc0 = Some IHalt-> 
+       tr_expr G pc0 1 Eexit 
+
+Either it: 
+  - executes from start to end, obeying stack expectations and producing aa suitable value in RA
+  - (if Eexit): it halts immediately
+
+
+*)
+
+
+(* Some basic definitions. *)
+
+
+
+Section WithMN.
+
+Require Import Lib.Monads.
+Import MonadNotations.
+Open Scope monad_scope.
+
+
+Definition code_at (G: Intermediate.GlobalEnv.global_env) (pc: Pointer.t) : option instr := 
+  do C_procs <- PMap.find (Pointer.component pc) (Intermediate.GlobalEnv.genv_procedures G);
+  do P_code <- PMap.find (Pointer.block pc) C_procs;
+  if Pointer.offset pc <? 0 then
+    None
+  else
+    nth_error P_code (Z.to_nat (Pointer.offset pc))
+.
+
+(*Lemma code_at_app:
+  forall i c2 c1 pc,
+  pc = length c1 ->
+  code_at (c1 ++ i :: c2) pc = Some i.
+Proof.
+  induction c1; simpl; intros; subst pc; auto.
+Qed.
+ *)
+
+End WithMN.
+
+Inductive codeseq_at (G:Intermediate.GlobalEnv.global_env) : Pointer.t -> code -> Prop :=
+  | codeseq_at_intro: forall C_procs C1 C2 C3 pc,
+      PMap.find (Pointer.component pc) (Intermediate.GlobalEnv.genv_procedures G) = Some C_procs ->
+      PMap.find (Pointer.block pc) C_procs = Some (C1 ++ C2 ++ C3) ->
+      Z.to_nat (Pointer.offset pc) = length C1 ->
+      codeseq_at G pc C2.
+
+(* ?? how do we handle compiling single expressions within the overall monadic structure? *)
+
+(* only next label matters; we will need to parameterize by that somehow *)
+Inductive expr_codeseq_at (G: Intermediate.GlobalEnv.global_env) : Pointer.t -> code -> expr -> Prop :=
+  | expr_codeseq_at_intro: forall C comp_env pc e,
+      run comp_env (compile_expr e) = Some C ->  (* BOGUS *)
+      codeseq_at G pc C ->
+      expr_codeseq_at G pc C e.
+
+
+Inductive compile_cont (G: Intermediate.GlobalEnv.global_env) : cont -> Pointer.t -> Prop :=
+  | ccont_binop1 : forall b e k C pc pc',
+      expr_codeseq_at G pc C e -> 
+      pc' = Pointer.add pc (Z.of_nat (length C + 1)) -> 
+      compile_cont G k pc' ->                                              
+      compile_cont G (Kbinop1 b e k) pc
+  | ccont_binop2 : forall b v k pc pc',
+      pc' = Pointer.add pc 2%Z -> 
+      compile_cont G k pc' ->                                              
+      compile_cont G (Kbinop2 b v k) pc
+  | ccont_seq : forall e k C pc pc',
+      expr_codeseq_at G pc C e -> 
+      pc' = Pointer.add pc (Z.of_nat (length C)) -> 
+      compile_cont G (Kseq e k) pc.
+(*  | ccont_if :
+      codeseq_at G pc [IBnz R_COM l1] ->  
+      codeseq_at G 
+      pc' = Pointer.add pc (Z.of_nat (length Ct + length Cf + 4)) -> 
+      compile_cont G (Kif et ef) pc.
+  
+| Kseq (e: expr) (k: cont)
+| Kif (e1: expr) (e2: expr) (k: cont)
+| Kalloc (k: cont)
+| Kderef (k: cont)
+| Kassign1 (e: expr) (k: cont)
+| Kassign2 (v: value) (k: cont)
+| Kcall (C: Component.id) (P: Procedure.id) (k: cont).
+ *)
+
+
+Inductive match_config (SG: Source.GlobalEnv.global_env) (IG: Intermediate.GlobalEnv.global_env): S.CS.state -> I.CS.state -> Prop :=
+  | match_config_intro: forall comp C s mem k e gps regs pc,
+      expr_codeseq_at IG pc C e -> 
+      compile_cont IG k (Pointer.add pc (Z.of_nat (length C))) -> 
+      (* some matching condintion on SG IG *)
+      match_config SG IG (comp, s, mem, k, e) (gps, mem, regs, pc).
+
+Ltac inv H := (inversion H; subst; clear H). 
+
+About CompMonad.Comp.bind.
+
+Remark bind_inversion:
+  forall (env A B: Type) (f: CompMonad.Comp.t env A) (g: A -> CompMonad.Comp.t env B) (y: B) (e e':env),
+  CompMonad.Comp.bind env _ _ f g e = Some (y,e') ->
+  exists x, f = Some x /\ g x = Some y.
+Proof.
+  intros until y. destruct f; simpl; intros.
+  exists a; auto.
+  discriminate.
+Qed.
+
+
+(*
+
+Ltac monadInv1 H :=
+  match type of H with
+  | (Some _ = Some _) =>
+      inversion H; clear H; try subst
+  | (None = Some _) => 
+      discriminate
+  | (CompMonad.Comp.bind ?F ?G = OK ?X) =>
+      let x := fresh "x" in (
+      let EQ1 := fresh "EQ" in (
+      let EQ2 := fresh "EQ" in (
+      destruct (bind_inversion F G H) as [x [EQ1 EQ2]];
+      clear H;
+      try (monadInv1 EQ2))))
+  | (bind2 ?F ?G = OK ?X) =>
+      let x1 := fresh "x" in (
+      let x2 := fresh "x" in (
+      let EQ1 := fresh "EQ" in (
+      let EQ2 := fresh "EQ" in (
+      destruct (bind2_inversion F G H) as [x1 [x2 [EQ1 EQ2]]];
+      clear H;
+      try (monadInv1 EQ2)))))
+  | (match ?X with left _ => _ | right _ => assertion_failed end = OK _) =>
+      destruct X; [try (monadInv1 H) | discriminate]
+  | (match (negb ?X) with true => _ | false => assertion_failed end = OK _) =>
+      destruct X as [] eqn:?; [discriminate | try (monadInv1 H)]
+  | (match ?X with true => _ | false => assertion_failed end = OK _) =>
+      destruct X as [] eqn:?; [try (monadInv1 H) | discriminate]
+  | (mmap ?F ?L = OK ?M) =>
+      generalize (mmap_inversion F L H); intro
+  end.
+
+Ltac monadInv H :=
+  monadInv1 H ||
+  match type of H with
+  | (?F _ _ _ _ _ _ _ _ = OK _) => 
+      ((progress simpl in H) || unfold F in H); monadInv1 H
+  | (?F _ _ _ _ _ _ _ = OK _) => 
+      ((progress simpl in H) || unfold F in H); monadInv1 H
+  | (?F _ _ _ _ _ _ = OK _) => 
+      ((progress simpl in H) || unfold F in H); monadInv1 H
+  | (?F _ _ _ _ _ = OK _) => 
+      ((progress simpl in H) || unfold F in H); monadInv1 H
+  | (?F _ _ _ _ = OK _) => 
+      ((progress simpl in H) || unfold F in H); monadInv1 H
+  | (?F _ _ _ = OK _) => 
+      ((progress simpl in H) || unfold F in H); monadInv1 H
+  | (?F _ _ = OK _) => 
+      ((progress simpl in H) || unfold F in H); monadInv1 H
+  | (?F _ = OK _) => 
+      ((progress simpl in H) || unfold F in H); monadInv1 H
+  end.
+ *)
+
+Lemma simulation_step:
+  forall SG IG sstate1 sstate2 istate1 t,
+  S.CS.kstep SG sstate1 t sstate2 ->
+  match_config SG IG sstate1 istate1 -> 
+  exists istate2,
+      star (I.CS.sem tp).(step) IG istate1 t istate2
+(*       (plus (transition C) machstate1 machstate2
+       \/ (star (transition C) machstate1 machstate2 /\ measure impstate2 < measure impstate1)) *)
+   /\ match_config SG IG sstate2 istate2.
+Proof.
+  intros until t; intros KSTEP MATCH. 
+  inversion KSTEP; clear KSTEP; subst; inversion MATCH; clear MATCH; subst; simpl in *.
+
+  - (* binop1 *)
+    econstructor; split.
+    apply star_refl. 
+    econstructor. 
+    inv H5. simpl in H. unfold run in H. 
+    destruct (        CompMonad.Comp.bind Compiler.comp_env code (list instr) (compile_expr e1)
+          (fun c1 : code =>
+           CompMonad.Comp.bind Compiler.comp_env code (list instr) (compile_expr e2)
+             (fun c2 : code =>
+              CompMonad.Comp.ret Compiler.comp_env (list instr)
+                (c1 ++
+                 IStore R_SP R_COM
+                 :: IBinOp Add R_SP R_ONE R_SP
+                    :: c2 ++ [IBinOp Minus R_SP R_ONE R_SP; ILoad R_SP R_AUX1; IBinOp op R_AUX1 R_COM R_COM])))
+          comp_env) eqn:X; [|inv H]. 
+    destruct p0; inv H. 
+
+    destruct (CompMonad.Comp.bind Compiler.comp_env code (list instr) (compile_expr e1)
+           (fun c1 : code =>
+            CompMonad.Comp.bind Compiler.comp_env code (list instr) (compile_expr e2)
+              (fun c2 : code =>
+               CompMonad.Comp.ret Compiler.comp_env (list instr)
+                 (c1 ++
+                  IStore R_SP R_COM
+                  :: IBinOp Add R_SP R_ONE R_SP
+                     :: c2 ++ [IBinOp Minus R_SP R_ONE R_SP; ILoad R_SP R_AUX1; IBinOp op R_AUX1 R_COM R_COM])))
+           comp_env) eqn:?; inv X. 
+    destruct (CompMonad.Comp.bind Compiler.comp_env code (list instr) (compile_expr e1)
+            (fun c1 : code =>
+             CompMonad.Comp.bind Compiler.comp_env code (list instr) (compile_expr e2)
+               (fun c2 : code =>
+                CompMonad.Comp.ret Compiler.comp_env (list instr)
+                  (c1 ++
+                   IStore R_SP R_COM
+                   :: IBinOp Add R_SP R_ONE R_SP
+                   :: c2 ++ [IBinOp Minus R_SP R_ONE R_SP; ILoad R_SP R_AUX1; IBinOp op R_AUX1 R_COM R_COM])))
+            comp_env) eqn: X; inv Heqo. 
+    destruct (CompMonad.Comp.bind Compiler.comp_env code (list instr) (compile_expr e1)
+           (fun c1 : code =>
+            CompMonad.Comp.bind Compiler.comp_env code (list instr) (compile_expr e2)
+              (fun c2 : code =>
+               CompMonad.Comp.ret Compiler.comp_env (list instr)
+                 (c1 ++
+                  IStore R_SP R_COM
+                  :: IBinOp Add R_SP R_ONE R_SP
+                     :: c2 ++ [IBinOp Minus R_SP R_ONE R_SP; ILoad R_SP R_AUX1; IBinOp op R_AUX1 R_COM R_COM])))
+           comp_env) eqn:?; inv X. 
+ CompMonad.Comp.bind Compiler.comp_env code (list instr) (compile_expr e1)
+           (fun c1 : code =>
+            CompMonad.Comp.bind Compiler.comp_env code (list instr) (compile_expr e2)
+              (fun c2 : code =>
+               CompMonad.Comp.ret Compiler.comp_env (list instr)
+                 (c1 ++
+                  IStore R_SP R_COM
+                  :: IBinOp Add R_SP R_ONE R_SP
+                     :: c2 ++ [IBinOp Minus R_SP R_ONE R_SP; ILoad R_SP R_AUX1; IBinOp op R_AUX1 R_COM R_COM])))
+           comp_env
+
+
+
+(* As a warm-up, some facts about stack use. *)
+
+Fixpoint stack_usage (e:expr) : nat :=
+  match e with
+  | E_val _ => 0
+  | E_local => 0
+  | E_binop _ e1 e2 => max (stack_usage e1) (1 + stack_usage e2)
+  | E_seq e1 e2 => max (stack_usage e1) (stack_usage e2)
+  | E_if e1 e2 e3 => max (stack_usage e1) (max (stack_usage e2) (stack_usage e3))
+  | E_alloc e0 => stack_usage e0
+  | E_deref e0 => stack_usage e0
+  | E_assign e1 e2 => max (stack_usage e1) (1 + stack_usage e2)
+  | E_call C P e0 => max (stack_usage e0) 2   (* subject to change? *)
+  | E_exit => 0
+  end.
+                         
+(* In reality, may want to prove this simultaneously with correctness... *)
+
+Import Intermediate.
+
+Lemma stack_usage_correct:
+  forall (e:expr) C G pc (m:nat) st mem regs sp sp' pc' st' mem' regs' t,
+  run init_env (compile_expr e) = Some C  ->  (* temporary -- nonsense? *)
+  codeseq_at G pc C -> 
+  stack_usage e = m -> 
+  Register.get R_SP regs = Ptr sp ->  
+  plus (I.CS.sem tp).(step) G (st,mem,regs,pc) t (st',mem',regs',pc') ->
+  Pointer.leq pc pc' = Some true ->
+  Pointer.leq pc' (Pointer.add pc (Z.of_nat (length C))) = Some true ->   
+  Register.get R_SP regs' = Ptr sp' -> 
+  Pointer.leq sp sp' = Some true /\ Pointer.leq sp' (Pointer.add sp (Z.of_nat m)) = Some true.
+Proof.
+  unfold run.
+  induction e; intros.
+  - destruct v; simpl in H; inv H. 
+    + simpl in H5.
+      inv H3. 
+      inv H1. 
+      * (* one step *)
+        rewrite <- I.CS.eval_step_correct in H.  simpl in H. 
+        inv H0.  rewrite H1 in H. rewrite H3 in H. 
+        assert (Pointer.offset pc <? 0 = false). admit.
+        rewrite H0 in H. 
+        inv H0. inv H10.
+        destruct H0 as [CC [P1 [P2 [P3 P4]]]].
+        rewrite P1 in H.  inv H.  rewrite H1 in P2.  inv P2. 
+      inv H1. 
+
+  simpl in H. 
+
+*)
+    
 Theorem well_formedness_preservation:
   Intermediate.well_formed_program tp.
 Proof.
